extraction/Extr.v
@@ -5,4 +5,4 @@ Separate Extraction
   EffIR.prog0 EffIR.observe EffIR.run
   Samples.sample_delete Samples.sample_two Samples.sample_ret
   Samples.sample_neg Samples.sample_nested
-  Samples.sample_throw Samples.sample_guard5.
+  Samples.sample_throw Samples.sample_guard5 Samples.sample_env.
